src/program_proof/simplepb/pb_roapply_proof.v
@@ -1,0 +1,1194 @@
+From Perennial.base_logic Require Import lib.saved_prop.
+From Perennial.program_proof Require Import grove_prelude.
+From Goose.github_com.mit_pdos.gokv.simplepb Require Export pb.
+From Perennial.program_proof.simplepb Require Import pb_ghost.
+From Perennial.goose_lang.lib Require Import waitgroup.
+From iris.base_logic Require Export lib.ghost_var mono_nat.
+From iris.algebra Require Import dfrac_agree mono_list.
+From Perennial.goose_lang Require Import crash_borrow.
+From Perennial.program_proof.simplepb Require Import pb_definitions pb_marshal_proof pb_applybackup_proof.
+From Perennial.program_proof.reconnectclient Require Import proof.
+
+Section pb_apply_proof.
+
+Context `{!heapGS Σ}.
+Context {pb_record:PBRecord}.
+
+Notation OpType := (pb_OpType pb_record).
+Notation has_op_encoding := (pb_has_op_encoding pb_record).
+Notation compute_reply := (pb_compute_reply pb_record).
+Notation pbG := (pbG (pb_record:=pb_record)).
+
+Context `{!pbG Σ}.
+
+Lemma wp_Clerk__ApplyRo γ γsys γsrv ck op_sl q op (op_bytes:list u8) (Φ:val → iProp Σ) :
+has_op_encoding op_bytes op →
+is_Clerk ck γsys γsrv -∗
+is_inv γ γsys -∗
+is_slice_small op_sl byteT q op_bytes -∗
+□((|={⊤∖↑pbN,∅}=> ∃ ops, own_log γ ops ∗
+  (own_log γ ops ={∅,⊤∖↑pbN}=∗
+     (∀ reply_sl, is_slice_small reply_sl byteT 1 (compute_reply ops op) -∗
+            is_slice_small op_sl byteT q op_bytes -∗
+                Φ (#(U64 0), slice_val reply_sl)%V)))
+∗
+(∀ (err:u64) unused_sl, ⌜err ≠ 0⌝ -∗ is_slice_small op_sl byteT q op_bytes -∗
+                                     Φ (#err, (slice_val unused_sl))%V )) -∗
+WP Clerk__ApplyRo #ck (slice_val op_sl) {{ Φ }}.
+Proof.
+  intros Henc.
+  iIntros "#Hck #Hinv Hop_sl".
+  iIntros "#HΦ".
+  wp_call.
+  wp_apply (wp_ref_of_zero).
+  { done. }
+  iIntros (rep) "Hrep".
+  wp_pures.
+  iNamed "Hck".
+  wp_loadField.
+  rewrite is_pb_host_unfold.
+  iNamed "Hsrv".
+  wp_apply (wp_ReconnectingClient__Call2 with "Hcl_rpc [] Hop_sl Hrep").
+  {
+    iDestruct "Hsrv" as "(_ & _ & _ & _ & _ & _ & $ & _)".
+  }
+  { (* Successful RPC *)
+    iModIntro.
+    iNext.
+    unfold Apply_spec.
+    iExists _, _.
+    iSplitR; first done.
+    iSplitR; first done.
+    simpl.
+    iSplit.
+    {
+      iModIntro.
+      iLeft in "HΦ".
+      iMod "HΦ".
+      iModIntro.
+      iDestruct "HΦ" as (?) "[Hlog HΦ]".
+      iExists _.
+      iFrame.
+      iIntros "Hlog".
+      iMod ("HΦ" with "Hlog") as "HΦ".
+      iModIntro.
+      iIntros (? Hreply_enc) "Hop".
+      iIntros (?) "Hrep Hrep_sl".
+      wp_pures.
+      wp_load.
+      rewrite Hreply_enc.
+      wp_apply (ApplyReply.wp_Decode with "[Hrep_sl]").
+      { iFrame. iPureIntro. done. }
+      iIntros (reply_ptr) "Hreply".
+      wp_pures.
+      iNamed "Hreply".
+      wp_loadField.
+      wp_loadField.
+      wp_pures.
+      iModIntro.
+      iApply ("HΦ" with "Hrepy_ret_sl Hop").
+    }
+    { (* Apply failed for some reason, e.g. node is not primary *)
+      iIntros (??).
+      iModIntro.
+      iIntros (Herr_nz ? Hreply_enc) "Hop".
+      iIntros (?) "Hrep Hrep_sl".
+      wp_pures.
+      iIntros.
+      wp_pures.
+      wp_load.
+      wp_apply (ApplyReply.wp_Decode with "[$Hrep_sl]").
+      { done. }
+      iIntros (reply_ptr) "Hreply".
+      iNamed "Hreply".
+      wp_pures.
+      wp_loadField.
+      wp_loadField.
+      iRight in "HΦ".
+      wp_pures.
+      iApply ("HΦ" with "[] Hop").
+      done.
+    }
+  }
+  { (* RPC error *)
+    iIntros.
+    wp_pures.
+    wp_if_destruct.
+    {
+      wp_load.
+      exfalso. done.
+    }
+    iRight in "HΦ".
+    replace (slice.nil) with (slice_val Slice.nil) by done.
+    wp_pures.
+    iApply ("HΦ" with "[] [$]").
+    done.
+  }
+Qed.
+
+Lemma wp_Server__RoApply_internal (s:loc) γ γsrv op_sl op_bytes op Q :
+  {{{
+        is_Server s γ γsrv ∗
+        readonly (is_slice_small op_sl byteT 1 op_bytes) ∗
+        ⌜has_op_encoding op_bytes op⌝ ∗
+        (|={⊤∖↑ghostN,∅}=> ∃ σ, own_ghost γ σ ∗ (own_ghost γ (σ ++ [(ro_op op, Q)]) ={∅,⊤∖↑ghostN}=∗ True))
+  }}}
+    pb.Server__ApplyRo #s (slice_val op_sl)
+  {{{
+        reply_ptr reply, RET #reply_ptr; £ 1 ∗ £ 1 ∗ £ 1 ∗ ApplyReply.own_q reply_ptr reply ∗
+        if (decide (reply.(ApplyReply.err) = 0%Z)) then
+          ∃ opsfull,
+            let ops := (get_rwops opsfull) in
+            ⌜reply.(ApplyReply.ret) = compute_reply ops op⌝ ∗
+            is_ghost_lb γ (opsfull ++ [(ro_op op, Q)])
+        else
+          True
+  }}}
+  .
+Proof.
+  iIntros (Φ) "[#His Hpre] HΦ".
+  iDestruct "Hpre" as "(#Hsl & %Hghostop_op & Hupd)".
+  iNamed "His".
+  rewrite /Server__ApplyRo.
+  wp_pure1_credit "Hcred3".
+  wp_pure1_credit "Hcred2".
+  wp_pure1_credit "Hcred1".
+  wp_apply (wp_allocStruct).
+  { eauto. }
+  iIntros (reply_ptr) "Hreply".
+  iDestruct (struct_fields_split with "Hreply") as "HH".
+  iNamed "HH".
+  wp_pure1_credit "Hlc1".
+  wp_pure1_credit "Hlc2".
+  simpl.
+  replace (slice.nil) with (slice_val (Slice.nil)) by done.
+  wp_storeField.
+
+  wp_loadField.
+  wp_apply (acquire_spec with "HmuInv").
+  iIntros "[Hlocked Hown]".
+  iNamed "Hown".
+  wp_pures.
+  wp_loadField.
+  wp_if_destruct.
+  { (* return error "not primary" *)
+    wp_loadField.
+    wp_apply (release_spec with "[-HΦ Err Reply Hcred1 Hcred2 Hcred3]").
+    {
+      iFrame "HmuInv Hlocked".
+      iNext.
+      repeat (iExists _).
+      iFrame "Hstate ∗#"; iFrame "%".
+    }
+    wp_pures.
+    wp_storeField.
+    iApply "HΦ".
+    iFrame.
+    iSplitL "Err Reply".
+    {
+      instantiate (1:=(ApplyReply.mkC _ _)).
+      iExists _.
+      iFrame.
+      iExists 1%Qp.
+      iApply is_slice_small_nil.
+      done.
+    }
+    done.
+  }
+  wp_loadField.
+
+  wp_if_destruct.
+  { (* return ESealed *)
+    wp_loadField.
+    wp_apply (release_spec with "[-HΦ Err Reply Hcred1 Hcred2 Hcred3]").
+    {
+      iFrame "HmuInv Hlocked".
+      iNext.
+      repeat (iExists _).
+      iFrame "∗#"; iFrame "%".
+    }
+    wp_pures.
+    wp_storeField.
+    iApply ("HΦ" $! _ (ApplyReply.mkC 1 [])).
+    iFrame.
+    iExists _, 1%Qp; iFrame.
+    iApply is_slice_small_nil.
+    done.
+  }
+
+  clear Heqb.
+
+  (* make proposal *)
+  iAssert (_) with "HprimaryOnly" as "HprimaryOnly2".
+  iEval (rewrite /is_possible_Primary /tc_opaque) in "HprimaryOnly2".
+  iNamed "HprimaryOnly2".
+  iAssert (_) with "HisSm" as "HisSm2".
+  iEval (rewrite /is_StateMachine /tc_opaque) in "HisSm2".
+  iNamed "HisSm2".
+  wp_loadField.
+  wp_loadField.
+
+  (* make ephemeral proposal first *)
+  iMod (own_update with "Heph") as "Heph".
+  {
+    apply singleton_update.
+    apply mono_list_update.
+    instantiate (1:=opsfull_ephemeral ++ [(ro_op op, Q)]).
+    by apply prefix_app_r.
+  }
+  iDestruct (own_mono _ _ {[ _ := ◯ML _ ]} with "Heph") as "#Hnew_eph_lb".
+  {
+    apply singleton_mono.
+    apply mono_list_included.
+  }
+
+  iApply fupd_wp.
+  iMod (fupd_mask_subseteq (↑pbN)) as "Hmask".
+  { set_solver. }
+  iMod (valid_add with "Hcred2 Heph_valid [Hupd]") as "#Hnew_eph_valid".
+  {
+    iMod "Hupd" as (?) "[Hghost Hupd]".
+    iModIntro.
+    iExists _; iFrame.
+    iIntros. done.
+  }
+  iMod "Hmask".
+  iModIntro.
+
+  (* NOTE: unlike Apply(), don't (and actually *can't* ) need to add to own_proposal. It is enough to
+     add to ephemeral_proposal. The applyRoThread() will handle appending to
+     own_proposal.
+   *)
+  wp_apply ("HapplyReadonlySpec" with "[HisSm $Hstate $Hsl]").
+  { done. }
+  iIntros (reply_sl q) "(Hreply & Hstate)".
+
+  wp_storeField.
+  wp_loadField.
+  wp_apply (std_proof.wp_SumAssumeNoOverflow).
+  iIntros "%Hno_overflow".
+  wp_storeField.
+  wp_loadField.
+  wp_pures.
+  wp_loadField.
+  wp_pures.
+  wp_loadField.
+  wp_pures.
+  wp_loadField.
+  wp_loadField.
+  wp_pures.
+  (* Possibly wake up the applyRoThread background goroutine, only if the
+     current nextIndex is durable *)
+  wp_apply (wp_If_optional with "[] [HroOpsToPropose_cond]").
+  2:{
+    iNamedAccu.
+  }
+  {
+    iIntros (?).
+    iNamed 1. iIntros "HΦ".
+    wp_loadField.
+    wp_apply (wp_condSignal with "[]").
+    { iFrame "#". }
+    by iApply "HΦ".
+  }
+  iNamed 1.
+
+  wp_pures.
+
+  (* Wait for the background thread to do the committing *)
+  iAssert (pb_definitions.own_Server s γ γsrv γeph _ mu) with "[-HΦ Hlc1 Hlc2]" as "Hown".
+  {
+    repeat iExists _.
+    iFrame "Hsealed Heph".
+    replace (get_rwops (opsfull_ephemeral ++ [(ro_op op, Q)])) with (get_rwops (opsfull_ephemeral)); last first.
+    {
+      rewrite get_rwops_app.
+      unfold get_rwops.
+      simpl.
+      rewrite app_nil_r.
+      done.
+    }
+    iFrame "∗".
+    iFrame "#".
+    iFrame "%".
+
+    (* establish new is_possible_Primary, because we increased nextRoIndex *)
+    repeat iExists _.
+    iFrame "Hcommit_lb #".
+    iFrame "%".
+    iPureIntro.
+    destruct Heph_proposal as (opsfull_eph_ro & Hsuffix & HnextRoIndex & HroOnly).
+    exists (opsfull_eph_ro ++ [(ro_op op, Q)]).
+    split.
+    {
+      apply suffix_app.
+      { done. }
+    }
+    split.
+    {
+      rewrite app_length.
+      simpl.
+      word.
+    }
+    rewrite get_rwops_app.
+    rewrite HroOnly.
+    simpl.
+    unfold get_rwops.
+    done.
+  }
+
+  wp_forBreak.
+
+  wp_pures.
+  iClear "Hs_epoch_lb HopAppliedConds_conds HdurableNextIndex_is_cond HroOpsToPropose_is_cond".
+  iClear "HcommittedNextRoIndex_is_cond Hdurable_lb Heph_prop_lb Hcommit_lb HprimaryOnly HisSm Heph_commit_lb Heph_valid".
+  iNamed "Hown".
+  wp_loadField.
+  wp_pures.
+  (* FIXME: compound condition in if statement... *)
+
+
+
+  (* reset nextRoIndex *)
+  wp_loadField.
+  wp_storeField.
+  wp_storeField.
+  wp_loadField.
+  replace (get_rwops opsfull_ephemeral ++ [op]) with (get_rwops (opsfull_ephemeral ++ [(rw_op op, Q)])); last first.
+  {
+    unfold get_rwops. rewrite map_app. rewrite concat_app.
+    done.
+  }
+  wp_apply (release_spec with "[-HΦ Hreply Err Reply Hlc1 Hlc2 HwaitSpec]").
+  {
+    iFrame "HmuInv Hlocked".
+    iNext.
+    repeat (iExists _).
+    iClear "Hnew_eph_lb".
+    iFrame "HisSm Hstate ∗ #"; iFrame "%".
+    iSplitR.
+    { iPureIntro.
+      rewrite get_rwops_app.
+      simpl.
+      rewrite app_length.
+      unfold get_rwops in *.
+      simpl.
+      word. }
+    unfold is_possible_Primary.
+    repeat iExists _.
+    iFrame "#"; iFrame "%".
+    iSplitR.
+    { iPureIntro. word. }
+    iSplitR.
+    { iPureIntro. intros. word. }
+    iSplitR.
+    {
+      iPureIntro.
+      exists [].
+      split.
+      { apply suffix_nil. }
+      split.
+      { simpl. word. }
+      { by unfold get_rwops. }
+    }
+    {
+      iPureIntro.
+      exists [].
+      split.
+      { apply suffix_nil. }
+      split.
+      { simpl. word. }
+      { by unfold get_rwops. }
+    }
+  }
+
+  wp_pures.
+
+  wp_apply "HwaitSpec".
+  iIntros "Hprimary_acc_lb".
+  iDestruct "Hprimary_acc_lb" as "(%Hσeq_phys & #Hprimary_acc_lb & #Hprop_lb & #Hprop_facts)".
+
+  wp_apply (wp_NewWaitGroup_free).
+  iIntros (wg) "Hwg".
+  wp_pures.
+
+  wp_apply (wp_allocStruct).
+  { econstructor; eauto. }
+  iIntros (Hargs) "Hargs".
+  iDestruct (struct_fields_split with "Hargs") as "HH".
+  iNamed "HH".
+  iMod (readonly_alloc_1 with "epoch") as "#Hargs_epoch".
+  iMod (readonly_alloc_1 with "index") as "#Hargs_index".
+  iMod (readonly_alloc_1 with "op") as "#Hargs_op".
+  wp_pures.
+  iMod (readonly_load with "Hclerkss_sl") as (?) "Hclerkss_sl2".
+
+  iDestruct (is_slice_small_sz with "Hclerkss_sl2") as %Hclerkss_sz.
+
+  wp_apply (wp_random).
+  iIntros (randint) "_".
+  wp_apply (wp_slice_len).
+  wp_pures.
+  set (clerkIdx:=(word.modu randint clerks_sl.(Slice.sz))).
+
+  assert (int.nat clerkIdx < length clerkss) as Hlookup_clerks.
+  {
+    rewrite Hclerkss_sz.
+    unfold clerkIdx.
+    rewrite Hclerkss_len in Hclerkss_sz.
+    replace (clerks_sl.(Slice.sz)) with (U64 (32)); last first.
+    {
+      unfold numClerks in Hclerkss_sz.
+      word.
+    }
+    enough (int.Z randint `mod` 32 < int.Z 32)%Z.
+    { word. }
+    apply Z.mod_pos_bound.
+    word.
+  }
+
+  assert (∃ clerks_sl_inner, clerkss !! int.nat clerkIdx%Z = Some clerks_sl_inner) as [clerks_sl_inner Hclerkss_lookup].
+  {
+    apply list_lookup_lt.
+    rewrite Hclerkss_len.
+    word.
+  }
+
+  wp_apply (wp_SliceGet with "[$Hclerkss_sl2]").
+  { done. }
+  iIntros "Hclerkss_sl2".
+  wp_pures.
+
+  wp_apply (wp_slice_len).
+  wp_apply (wp_new_slice).
+  { done. }
+  iIntros (errs_sl) "Herrs_sl".
+  wp_pures.
+  iApply fupd_wp.
+  iMod (fupd_mask_subseteq (↑pbN)) as "Hmask".
+  { set_solver. }
+  iMod (free_WaitGroup_alloc pbN _
+                             (λ i,
+                               ∃ (err:u64) γsrv',
+                               ⌜backups !! int.nat i = Some γsrv'⌝ ∗
+                               readonly ((errs_sl.(Slice.ptr) +ₗ[uint64T] int.Z i)↦[uint64T] #err) ∗
+                               □ if (decide (err = U64 0)) then
+                                 is_accepted_lb γsrv' epoch (opsfull_ephemeral ++ [_])
+                               else
+                                 True
+                             )%I
+         with "Hwg") as (γwg) "Hwg".
+  iMod "Hmask".
+  iModIntro.
+
+  iDestruct (big_sepL_lookup_acc with "Hclerkss_rpc") as "[Hclerks_rpc _]".
+  { done. }
+  iNamed "Hclerks_rpc".
+
+  iMod (readonly_load with "Hclerks_sl") as (?) "Hclerks_sl2".
+  wp_apply (wp_forSlice (λ j, (own_WaitGroup pbN wg γwg j _) ∗
+                              (errs_sl.(Slice.ptr) +ₗ[uint64T] int.Z j)↦∗[uint64T] (replicate (int.nat clerks_sl_inner.(Slice.sz) - int.nat j) #0)
+                        )%I with "[] [Hwg Herrs_sl $Hclerks_sl2]").
+  2: {
+    iSplitR "Herrs_sl".
+    { iExactEq "Hwg". econstructor. }
+    {
+      unfold slice.is_slice. unfold slice.is_slice_small.
+      iDestruct "Herrs_sl" as "[[Herrs_sl %Hlen] _]".
+      destruct Hlen as [Hlen _].
+      rewrite replicate_length in Hlen.
+      rewrite Hlen.
+      iExactEq "Herrs_sl".
+      simpl.
+      replace (1 * int.Z _)%Z with (0%Z) by word.
+      rewrite loc_add_0.
+      replace (int.nat _ - int.nat 0) with (int.nat errs_sl.(Slice.sz)) by word.
+      done.
+    }
+  }
+  {
+    iIntros (i ck).
+    clear Φ.
+    iIntros (Φ) "!# ([Hwg Herr_ptrs]& %Hi_ineq & %Hlookup) HΦ".
+    wp_pures.
+    wp_apply (wp_WaitGroup__Add with "[$Hwg]").
+    { word. }
+    iIntros "[Hwg Hwg_tok]".
+    wp_pures.
+    replace (int.nat clerks_sl_inner.(Slice.sz) - int.nat i) with (S (int.nat clerks_sl_inner.(Slice.sz) - (int.nat (word.add i 1)))); last first.
+    { word. }
+    rewrite replicate_S.
+    iDestruct (array_cons with "Herr_ptrs") as "[Herr_ptr Herr_ptrs]".
+    (* use wgTok to set errs_sl *)
+    iDestruct (own_WaitGroup_to_is_WaitGroup with "[$Hwg]") as "#His_wg".
+    wp_apply (wp_fork with "[Hwg_tok Herr_ptr]").
+    {
+      iNext.
+      iDestruct (big_sepL2_lookup_1_some with "Hclerks_rpc") as %[γsrv' Hlookupγ].
+      { done. }
+      iDestruct (big_sepL2_lookup_acc with "Hclerks_rpc") as "Hclerk_rpc".
+      { done. }
+      { done. }
+      iDestruct "Hclerk_rpc" as "[[Hclerk_rpc Hepoch_lb] _]".
+
+      wp_pures.
+      wp_forBreak_cond.
+      wp_pures.
+
+      wp_apply (wp_Clerk__ApplyAsBackup with "[$Hclerk_rpc $Hepoch_lb]").
+      {
+        iFrame "Hprop_lb Hprop_facts #".
+        iPureIntro.
+        rewrite last_app.
+        simpl.
+        split; eauto.
+        split; eauto.
+        split.
+        { rewrite get_rwops_app app_length. simpl.
+          word.
+        }
+        word.
+      }
+      iIntros (err) "#Hpost".
+
+      wp_pures.
+      destruct bool_decide.
+      {
+        wp_pures.
+        iLeft.
+        iFrame "∗".
+        by iPureIntro.
+      }
+      wp_if_destruct.
+      {
+        wp_pures.
+        iLeft.
+        iFrame "∗".
+        by iPureIntro.
+      }
+
+      unfold SliceSet.
+      wp_pures.
+      unfold slice.ptr.
+      wp_pures.
+      wp_store.
+      iRight.
+      iModIntro.
+      iSplitR; first by iPureIntro.
+
+      iMod (readonly_alloc_1 with "Herr_ptr") as "#Herr_ptr".
+      wp_apply (wp_WaitGroup__Done with "[$Hwg_tok $His_wg Herr_ptr Hpost]").
+      {
+        iModIntro.
+        iExists _, _.
+        iSplitL ""; first done.
+        iFrame "#".
+      }
+      done.
+    }
+    iApply "HΦ".
+    iFrame "Hwg".
+    iExactEq "Herr_ptrs".
+    f_equal.
+    rewrite /ty_size //=.
+    rewrite loc_add_assoc.
+    f_equal.
+    word.
+  }
+  iIntros "[[Hwg _] _]".
+  wp_pures.
+
+  wp_apply (wp_WaitGroup__Wait with "[$Hwg]").
+  iIntros "#Hwg_post".
+  wp_pures.
+  wp_apply (wp_ref_to).
+  { repeat econstructor. }
+  iIntros (err_ptr) "Herr".
+  wp_pures.
+
+  wp_apply (wp_ref_to).
+  { do 2 econstructor. }
+  iIntros (j_ptr) "Hi".
+  wp_pures.
+
+  set (conf:=(γsrv::backups)).
+  iAssert (∃ (j err:u64),
+              "Hj" ∷ j_ptr ↦[uint64T] #j ∗
+              "%Hj_ub" ∷ ⌜int.nat j ≤ length clerks⌝ ∗
+              "Herr" ∷ err_ptr ↦[uint64T] #err ∗
+              "#Hrest" ∷ □ if (decide (err = (U64 0)%Z)) then
+                (∀ (k:u64) γsrv', ⌜int.nat k ≤ int.nat j⌝ -∗ ⌜conf !! (int.nat k) = Some γsrv'⌝ -∗ is_accepted_lb γsrv' epoch (opsfull_ephemeral ++ [_]))
+              else
+                True
+          )%I with "[Hi Herr]" as "Hloop".
+  {
+    iExists _, _.
+    iFrame.
+    destruct (decide (_)).
+    {
+      iIntros.
+      iSplitL "".
+      { iPureIntro. word. }
+      iModIntro.
+      iIntros.
+      replace (int.nat 0%Z) with (0) in H by word.
+      replace (int.nat k) with (0) in H0 by word.
+      unfold conf in H0.
+      simpl in H0.
+      injection H0 as <-.
+      iFrame "Hprimary_acc_lb".
+    }
+    {
+      done.
+    }
+  }
+  wp_forBreak_cond.
+  wp_pures.
+  iNamed "Hloop".
+  wp_load.
+  wp_apply wp_slice_len.
+
+  iMod (readonly_load with "Hclerks_sl") as (?) "Htemp".
+  iDestruct (is_slice_small_sz with "Htemp") as %Hclerk_sz.
+  iClear "Htemp".
+
+  wp_pures.
+  wp_if_destruct.
+  {
+    wp_pures.
+    wp_load.
+    unfold SliceGet.
+    wp_call.
+    iDestruct (big_sepS_elem_of_acc _ _ j with "Hwg_post") as "[HH _]".
+    { set_solver. }
+    iDestruct "HH" as "[%Hbad|HH]".
+    { exfalso. word. }
+    iDestruct "HH" as (??) "(%HbackupLookup & Herr2 & Hpost)".
+    wp_apply (wp_slice_ptr).
+    wp_pure1.
+    iEval (simpl) in "Herr2".
+    iMod (readonly_load with "Herr2") as (?) "Herr3".
+    wp_load.
+    wp_pures.
+    destruct (bool_decide (_)) as [] eqn:Herr; wp_pures.
+    {
+      rewrite bool_decide_eq_true in Herr.
+      replace (err0) with (U64 0%Z) by naive_solver.
+      wp_pures.
+      wp_load; wp_store.
+      iLeft.
+      iModIntro.
+      iSplitL ""; first done.
+      iFrame "∗".
+      iExists _, _.
+      iFrame "Hj Herr".
+      iSplitL "".
+      { iPureIntro. word. }
+      iModIntro.
+      destruct (decide (err = 0%Z)).
+      {
+        iIntros.
+        assert (int.nat k ≤ int.nat j ∨ int.nat k = int.nat (word.add j 1%Z)) as [|].
+        {
+          replace (int.nat (word.add j 1%Z)) with (int.nat j + 1) in * by word.
+          word.
+        }
+        {
+          by iApply "Hrest".
+        }
+        {
+          destruct (decide (_)); last by exfalso.
+          replace (γsrv'0) with (γsrv'); last first.
+          {
+            rewrite H1 in H0.
+            replace (int.nat (word.add j 1%Z)) with (S (int.nat j)) in H0 by word.
+            unfold conf in H0.
+            rewrite lookup_cons in H0.
+            naive_solver.
+          }
+          iDestruct "Hpost" as "#$".
+        }
+      }
+      {
+        done.
+      }
+    }
+    {
+      wp_store.
+      wp_pures.
+      wp_load; wp_store.
+      iLeft.
+      iModIntro.
+      iSplitL ""; first done.
+      iFrame "∗".
+      iExists _, _.
+      iFrame "Hj Herr".
+      destruct (decide (err0 = _)).
+      { exfalso. naive_solver. }
+      iPureIntro.
+      word.
+    }
+  }
+  iRight.
+  iModIntro.
+  iSplitL ""; first done.
+  wp_pure1_credit "Hlc3".
+  wp_load.
+  wp_pures.
+
+  wp_storeField.
+  wp_load.
+
+  destruct (decide (err = 0%Z)); last first.
+  {
+    wp_pures.
+    rewrite bool_decide_false; last naive_solver.
+    wp_pures.
+    iApply ("HΦ" $! reply_ptr (ApplyReply.mkC _ _)).
+    iFrame.
+    simpl.
+    rewrite decide_False; last naive_solver.
+    iModIntro.
+    iSplitL; last done.
+    iExists _, _; iFrame.
+  }
+  (* otherwise, no error *)
+  iMod (ghost_commit with "Hsys_inv [Hrest] Hprop_lb Hprop_facts") as "#Hcommit".
+  {
+    iExists _; iFrame "#".
+    iIntros.
+    apply elem_of_list_lookup_1 in H as [k Hlookup_conf].
+    replace (int.nat j) with (length clerks); last first.
+    { word. }
+    epose proof (lookup_lt_Some _ _ _ Hlookup_conf) as HH.
+    replace (k) with (int.nat k) in *; last first.
+    {
+      rewrite cons_length in HH.
+      word.
+    }
+    iApply ("Hrest" $! k).
+    { iPureIntro.
+      unfold conf in HH.
+      rewrite cons_length in HH.
+      lia. }
+    { done. }
+  }
+
+  wp_pures.
+  rewrite bool_decide_true; last naive_solver.
+  wp_pures.
+  wp_loadField.
+  wp_apply (acquire_spec with "HmuInv").
+  iIntros "[Hlocked Hown]".
+  wp_pures.
+  iClear "Hs_epoch_lb HopAppliedConds_conds HdurableNextIndex_is_cond HroOpsToPropose_is_cond".
+  iClear "HcommittedNextRoIndex_is_cond Hdurable_lb Heph_prop_lb Hcommit_lb HprimaryOnly HisSm Heph_commit_lb Heph_valid".
+  iNamed "Hown".
+  wp_loadField.
+  wp_pures.
+  wp_apply (wp_and with "HcommittedNextIndex").
+  { wp_pures. iModIntro. iPureIntro. done. }
+  { iIntros. wp_loadField. wp_pures. iModIntro. iFrame.
+    done.
+  }
+  iIntros "HcommittedNextIndex".
+  wp_if_destruct.
+  {
+    destruct Heqb0 as [HepochEq HcommittedIneq].
+    injection HepochEq as H.
+    subst.
+    wp_storeField.
+    wp_loadField.
+    wp_apply (wp_condBroadcast with "[]").
+    { iFrame "#". }
+    wp_pures.
+    wp_loadField.
+    wp_apply (release_spec with "[-HΦ Hlc1 Hlc2 Hlc3 Hreply Err Reply]").
+    {
+      iFrame "Hlocked HmuInv".
+      iNext.
+      repeat iExists _.
+      iDestruct (own_valid_2 with "Heph Hnew_eph_lb") as %Hlenineq.
+      rewrite singleton_op singleton_valid in Hlenineq.
+      apply mono_list_both_valid_L in Hlenineq.
+      iFrame "∗ #"; iFrame "%".
+      rewrite /is_possible_Primary /tc_opaque.
+      iClear "Htok_used_witness Hconf Hclerkss_sl Hclerkss_rpc".
+      destruct isPrimary; last done.
+      iNamed "HprimaryOnly".
+      repeat iExists _.
+      iClear "Hcommit_lb".
+      time (iFrame "Hcommit #"; iFrame "%").
+
+      iPureIntro.
+
+      apply get_rwops_prefix in Hlenineq.
+      apply prefix_length in Hlenineq.
+      rewrite get_rwops_app app_length /= in Hlenineq.
+      rewrite Hσ_nextIndex in Hlenineq.
+      rewrite Hσ_nextIndex0 in Hlenineq.
+      split.
+      {
+        (* FIXME: why can't word to do this *)
+        rewrite Hno_overflow.
+        simpl.
+        replace (Z.to_nat (int.Z nextIndex + int.Z 1%Z)) with (int.nat nextIndex + 1).
+        { word. }
+        rewrite Z2Nat.inj_add.
+        { replace (int.nat 1) with (1). { done. }
+          word. } (* FIXME: word slow? *)
+        { word. }
+        { word. }
+      }
+      split.
+      { intros. apply HcommitRoNz0.
+        clear H.
+        time word.
+        (* Argument:
+           s.committedNextIndex < opNextIndex.
+           nextIndex + 1 <= s.nextIndex
+           s.committedNextIndex <= s.nextIndex
+         *)
+        (*
+        revert dependent nextIndex0.
+        revert dependent nextIndex.
+        revert dependent committedNextIndex0.
+        clear.
+        intros.
+        replace (int.Z 1) with (1%Z) in Hno_overflow by word.
+        rewrite Hno_overflow in H.
+        rewrite Z2Nat.inj_add in H; try word.
+        replace (int.nat 1) with (1) in * by word.
+        assert (int.nat nextIndex < int.nat nextIndex + int.nat 1) by word.
+        word.
+        clear -nextIndex0
+        *)
+      }
+      split.
+      { rewrite get_rwops_app app_length. simpl. time word. }
+      {
+        exists []. split.
+        { apply suffix_nil. }
+        split.
+        { simpl. (* FIXME: op_commit_ro is relative to committedNextIndex,
+                    whereas the code treats it as relavite to nextIndex. *)
+          symmetry.
+          apply HcommitRoNz0.
+          clear Hclerkss_len.
+          time word. }
+        { by unfold get_rwops. }
+      }
+    }
+    wp_pures.
+    iModIntro.
+    iApply ("HΦ" $! reply_ptr (ApplyReply.mkC _ _)).
+    iFrame "Hlc1 Hlc2 Hlc3".
+    iSplitL.
+    { iExists _, _. iFrame. }
+    simpl.
+    destruct (decide _); last first.
+    { exfalso. done. }
+    iExists _; iFrame "Hcommit".
+    done.
+  }
+
+  wp_loadField.
+  wp_apply (release_spec with "[-HΦ Hlc1 Hlc2 Hlc3 Hreply Err Reply]").
+  {
+    iFrame "Hlocked HmuInv".
+    iNext.
+    repeat iExists _.
+    iFrame "∗#"; iFrame "%".
+  }
+  wp_pures.
+  iModIntro.
+  iApply ("HΦ" $! reply_ptr (ApplyReply.mkC _ _)).
+  simpl.
+  iFrame "Hlc1 Hlc2 Hlc3".
+  iSplitL.
+  {
+    iExists _, _; iFrame.
+  }
+  destruct (decide _); last first.
+  { exfalso. done. }
+  iExists _.
+  iFrame "Hcommit".
+  done.
+Qed.
+
+Lemma prefix_app_cases {A} (σ σ':list A) e:
+  σ' `prefix_of` σ ++ [e] →
+  σ' `prefix_of` σ ∨ σ' = (σ++[e]).
+Proof.
+  intros [σ0 Heq].
+  induction σ0 using rev_ind.
+  { rewrite app_nil_r in Heq. right; congruence. }
+  { rewrite app_assoc in Heq.
+    apply app_inj_2 in Heq as [-> ?]; last auto.
+    left. eexists; eauto.
+  }
+Qed.
+
+Lemma get_rwops_fst {A B} ops1 ops2 :
+  ops1.*1 = ops2.*1 →
+  get_rwops (A:=A) (pb_record:=pb_record) ops1 = get_rwops (A:=B) (pb_record:=pb_record) ops2.
+Proof.
+  intros.
+  revert dependent ops2.
+  induction ops1.
+  {
+    intros.
+    simpl.
+    destruct ops2.
+    { done. }
+    by exfalso.
+  }
+  intros.
+  revert dependent IHops1.
+  induction ops2; intros.
+  { by exfalso. }
+  replace (a :: ops1) with ([a] ++ ops1) in * by done.
+  replace (a0 :: ops2) with ([a0] ++ ops2) in * by done.
+  repeat rewrite get_rwops_app.
+  repeat rewrite fmap_app in H.
+  apply app_inj_1 in H; last done.
+  destruct H as [Hfirst Hrest].
+  injection Hfirst as Hfirst.
+  erewrite IHops1; last done.
+  f_equal.
+  destruct a, a0.
+  simpl in *.
+  unfold get_rwops.
+  simpl.
+  subst.
+  done.
+Qed.
+
+Lemma wp_Server__Apply (s:loc) γlog γ γsrv op_sl op (enc_op:list u8) Ψ (Φ: val → iProp Σ) :
+  is_Server s γ γsrv -∗
+  readonly (is_slice_small op_sl byteT 1 enc_op) -∗
+  (∀ reply, Ψ reply -∗ ∀ reply_ptr, ApplyReply.own_q reply_ptr reply -∗ Φ #reply_ptr) -∗
+  Apply_core_spec γ γlog op enc_op Ψ -∗
+  WP (pb.Server__Apply #s (slice_val op_sl)) {{ Φ }}
+.
+Proof using Type*.
+  iIntros "#Hsrv #Hop_sl".
+  iIntros "HΨ HΦ".
+  iApply (wp_frame_wand with "HΨ").
+  iDestruct "HΦ" as "(%Hop_enc & #Hinv & #Hupd & Hfail_Φ)".
+  iMod (ghost_var_alloc (())) as (γtok) "Htok".
+  set (OpPred :=
+(λ ops, inv escrowN (
+        Ψ (ApplyReply.mkC 0 (compute_reply ops op)) ∨
+          ghost_var γtok 1 ()
+        ))).
+
+  iMod (saved_pred_alloc OpPred DfracDiscarded) as (γghost_op) "#Hsaved"; first done.
+  iApply wp_fupd.
+  wp_apply (wp_Server__Apply_internal _ _ _ _ _
+      op γghost_op
+             with "[$Hsrv $Hop_sl Hupd]").
+  {
+    iSplitL ""; first done.
+    iInv "Hinv" as "HH" "Hclose".
+    iDestruct "HH" as (?) "(Hghost & >Hlog & #HQs)".
+    iDestruct "Hghost" as (σgnames) "(>Hghost&>%Hfst_eq&#Hsaved')".
+    iMod (fupd_mask_subseteq (⊤∖↑pbN)) as "Hmask".
+    {
+      assert ((↑ghostN:coPset) ⊆ (↑pbN:coPset)).
+      { apply nclose_subseteq. }
+      assert ((↑appN:coPset) ⊆ (↑pbN:coPset)).
+      { apply nclose_subseteq. }
+      set_solver.
+    }
+    iMod "Hupd".
+    iModIntro.
+    iDestruct "Hupd" as (σ0) "[Hlog2 Hupd]".
+    iDestruct (own_valid_2 with "Hlog Hlog2") as %Hvalid.
+    apply mono_list_auth_dfrac_op_valid_L in Hvalid.
+    destruct Hvalid as [_ <-].
+    iExists _; iFrame.
+    iIntros "Hghost".
+    iMod (own_update_2 with "Hlog Hlog2") as "Hlog".
+    {
+      rewrite -mono_list_auth_dfrac_op.
+      rewrite dfrac_op_own.
+      rewrite Qp.half_half.
+      apply mono_list_update.
+      instantiate (1:=_ ++ [op]).
+      by apply prefix_app_r.
+    }
+    iEval (rewrite -Qp.half_half -dfrac_op_own mono_list_auth_dfrac_op) in "Hlog".
+    iDestruct "Hlog" as "[Hlog Hlog2]".
+    iMod ("Hupd" with "Hlog2") as "Hupd".
+
+    iAssert (|={↑escrowN}=> inv escrowN ((Ψ (ApplyReply.mkC 0 (compute_reply (get_rwops opsfullQ) op)))
+                                  ∨ ghost_var γtok 1 ()))%I
+            with "[Hupd]" as "Hinv2".
+    {
+      iMod (inv_alloc with "[-]") as "$"; last done.
+      iNext.
+      iIntros.
+      iLeft.
+      iIntros.
+      iApply "Hupd".
+    }
+    iMod "Hmask" as "_".
+    iMod (fupd_mask_subseteq (↑escrowN)) as "Hmask".
+    {
+      assert ((↑escrowN:coPset) ## (↑ghostN:coPset)).
+      { by apply ndot_ne_disjoint. }
+      assert ((↑escrowN:coPset) ## (↑appN:coPset)).
+      { by apply ndot_ne_disjoint. }
+      set_solver.
+    }
+    iMod "Hinv2" as "#HΦ_inv".
+    iMod "Hmask".
+
+    iMod ("Hclose" with "[HQs Hghost Hlog]").
+    {
+      iNext.
+      iExists (opsfullQ ++ [(rw_op op, OpPred)]); iFrame.
+      iSplitL "Hghost".
+      { iExists _. iFrame.
+        iSplitL.
+        { iPureIntro. rewrite ?fmap_app /=. congruence. }
+        rewrite ?fmap_app. iApply big_sepL2_app.
+        { iFrame "Hsaved'". }
+        iApply big_sepL2_singleton. iFrame "Hsaved".
+      }
+      rewrite get_rwops_app.
+      iFrame.
+
+      iModIntro.
+      iIntros.
+      apply prefix_app_cases in H as [Hprefix_of_old|Hnew].
+      {
+        iApply "HQs".
+        { done. }
+        { done. }
+      }
+      {
+        rewrite Hnew in H0.
+        assert (opsfullQ = opsPrePre) as ->.
+        { (* TODO: list_solver. *)
+          apply (f_equal reverse) in H0.
+          rewrite reverse_snoc in H0.
+          rewrite reverse_snoc in H0.
+          inversion H0.
+          apply (f_equal reverse) in H2.
+          rewrite reverse_involutive in H2.
+          rewrite reverse_involutive in H2.
+          done.
+        }
+        eassert (_ = lastEnt) as <-.
+        { eapply (suffix_snoc_inv_1 _ _ _ opsPrePre). rewrite -H0.
+          done. }
+        simpl.
+        unfold OpPred.
+        iFrame "#".
+      }
+    }
+    done.
+  }
+  iIntros (err reply).
+  iIntros "(Hcred & Hcred2 & Hcred3 & Hreply & Hpost)".
+  destruct (decide (reply.(ApplyReply.err) = U64 0)).
+  { (* no error *)
+    iNamed "Hreply".
+    rewrite e.
+    iDestruct "Hpost" as (?) "[%Hrep #Hghost_lb]".
+    rewrite Hrep.
+    iInv "Hinv" as "HH" "Hclose".
+    {
+      iDestruct "HH" as (?) "(Hghost & >Hlog & #HQs)".
+      iDestruct "Hghost" as (σgnames) "(>Hghost&>%Hfst_eq&#Hsaved')".
+      iApply (lc_fupd_add_later with "Hcred").
+      iNext.
+      iDestruct (own_valid_2 with "Hghost Hghost_lb") as %Hvalid.
+      rewrite mono_list_both_dfrac_valid_L in Hvalid.
+      destruct Hvalid as [_ Hvalid].
+
+      destruct Hvalid as (σtail&Hvalid').
+      subst.
+      iDestruct (big_sepL2_length with "Hsaved'") as %Hlen.
+      rewrite ?fmap_length in Hlen.
+      assert (∃ σ0a op' Q' σ0b,
+                 opsfullQ = σ0a ++ [(op', Q')] ++ σ0b ∧
+                 length σ0a = length opsfull ∧
+                 length σ0b = length σtail) as (σ0a&op'&Q'&σ0b&Heq0&Hlena&Hlenb).
+      {
+
+        destruct (nth_error opsfullQ (length opsfull)) as [(op', Q')|] eqn:Hnth; last first.
+        { apply nth_error_None in Hnth. rewrite ?app_length /= in Hlen. lia. }
+        edestruct (nth_error_split opsfullQ (length opsfull)) as (l1&l2&Heq&Hlen'); eauto.
+        eexists l1, _, _, l2. rewrite Heq /=; split_and!; eauto.
+        rewrite Heq ?app_length /= in Hlen. rewrite Hlen' in Hlen. clear -Hlen.
+        (* weird, lia fails directly but if you replace lengths with a nat then it works... *)
+        remember (length l2) as k.
+        remember (length σtail) as k'. rewrite Heqk in Hlen. rewrite -Heqk' in Hlen. lia.
+      }
+
+      iDestruct ("HQs" $! (σ0a ++ [(op', Q')]) _ (_, _) with "[] []") as "#HQ".
+      { rewrite Heq0. iPureIntro; eexists; eauto. rewrite app_assoc.  done. }
+      { done. }
+      simpl.
+      iMod ("Hclose" with "[Hghost Hlog]") as "_".
+      {
+        iNext.
+        iExists _; iFrame "∗#".
+        iExists _. iFrame.
+        iSplit.
+        { iPureIntro. auto. }
+        iApply "Hsaved'".
+      }
+
+      rewrite Heq0. rewrite ?fmap_app -app_assoc. iDestruct (big_sepL2_app_inv with "Hsaved'") as "(H1&H2)".
+      { left. rewrite ?fmap_length //. }
+
+      iEval (simpl) in "H2". iDestruct "H2" as "(HsavedQ'&?)".
+      iDestruct (saved_pred_agree _ _ _ _  _ (get_rwops σ0a) with "Hsaved [$]") as "HQequiv".
+      iApply (lc_fupd_add_later with "[$]"). iNext.
+      iRewrite -"HQequiv" in "HQ".
+
+      iInv "HQ" as "Hescrow" "Hclose".
+      iDestruct "Hescrow" as "[HΦ|>Hbad]"; last first.
+      {
+        iDestruct (ghost_var_valid_2 with "Htok Hbad") as %Hbad.
+        exfalso. naive_solver.
+      }
+      iMod ("Hclose" with "[$Htok]").
+      iMod (lc_fupd_elim_later with "Hcred2 HΦ") as "HΦ".
+      iModIntro.
+      iIntros "HΨ".
+      iApply ("HΨ" with "HΦ").
+      iExists _, _.
+      iFrame.
+      simpl.
+      rewrite /named.
+      iExactEq "Hrepy_ret_sl".
+      { repeat f_equal.
+        rewrite Heq0 in Hfst_eq. rewrite ?fmap_app -app_assoc in Hfst_eq.
+        apply app_inj_1 in Hfst_eq; last (rewrite ?fmap_length //).
+        destruct Hfst_eq as (Hfst_eq&_).
+        apply (get_rwops_fst σ0a opsfull) in Hfst_eq as ->.
+        done.
+      }
+    }
+  }
+  {
+    iIntros.
+    iNamed "Hreply".
+    iModIntro.
+    iIntros "HΨ".
+    iApply ("HΨ" with "[Hfail_Φ]").
+    {
+      iApply "Hfail_Φ".
+      done.
+    }
+    iExists _, _.
+    iFrame.
+  }
+Qed.
+
+End pb_apply_proof.
